src-proof-test structure

w64x4/test/Fp_w64x4.c
@@ -1,0 +1,24 @@
+#include <stdio.h>
+#include <stdint.h>
+#include <assert.h>
+
+
+extern uint64_t* __addm(uint64_t* p, uint64_t* a, uint64_t* b);
+
+
+int main() {
+  uint64_t* r;
+
+  uint64_t x[4] = { 5ull, 0ull, 0ull, 0ull };
+  uint64_t y[4] = { 7ull, 0ull, 0ull, 0ull };
+  uint64_t result[4];
+ 
+  r = __addm(result, x, y);
+
+  printf("%lu\n", (*result));
+  printf("%lu\n", *(result + (sizeof(unsigned long)/sizeof(uint64_t))));
+
+  return 0;
+}
+
+
