w64x4/src/Fp_w64x4_extract.ec
@@ -89,12 +89,12 @@ module M = {
     var cf:bool;
     var i:int;
     
-    (aux, aux_0) <- addc_64 a.[0] b false;
+    (aux, aux_0) <- adc_64 a.[0] b false;
     cf <- aux;
     a.[0] <- aux_0;
     i <- 1;
     while (i < 4) {
-      (aux, aux_0) <- addc_64 a.[i] (W64.of_int 0) cf;
+      (aux, aux_0) <- adc_64 a.[i] (W64.of_int 0) cf;
       cf <- aux;
       a.[i] <- aux_0;
       i <- i + 1;
@@ -110,12 +110,12 @@ module M = {
     var cf:bool;
     var i:int;
     
-    (aux, aux_0) <- addc_64 a.[0] b.[0] false;
+    (aux, aux_0) <- adc_64 a.[0] b.[0] false;
     cf <- aux;
     a.[0] <- aux_0;
     i <- 1;
     while (i < 4) {
-      (aux, aux_0) <- addc_64 a.[i] b.[i] cf;
+      (aux, aux_0) <- adc_64 a.[i] b.[i] cf;
       cf <- aux;
       a.[i] <- aux_0;
       i <- i + 1;
@@ -131,12 +131,12 @@ module M = {
     var cf:bool;
     var i:int;
     
-    (aux, aux_0) <- subc_64 a.[0] b.[0] false;
+    (aux, aux_0) <- sbb_64 a.[0] b.[0] false;
     cf <- aux;
     a.[0] <- aux_0;
     i <- 1;
     while (i < 4) {
-      (aux, aux_0) <- subc_64 a.[i] b.[i] cf;
+      (aux, aux_0) <- sbb_64 a.[i] b.[i] cf;
       cf <- aux;
       a.[i] <- aux_0;
       i <- i + 1;
@@ -242,11 +242,62 @@ module M = {
     return (_zero, of_0, cf, r);
   }
   
+  proc ith_bit64 (k:W64.t, ctr:W64.t) : W64.t = {
+    
+    var bit:W64.t;
+    var p:W64.t;
+    
+    bit <- k;
+    p <- ctr;
+    p <- (p `&` (W64.of_int 63));
+    bit <- (bit `>>` (truncateu8 p));
+    bit <- (bit `&` (W64.of_int 1));
+    return (bit);
+  }
+  
+  proc ith_bit (kk:W64.t Array4.t, ctr:W64.t) : W64.t = {
+    
+    var bit:W64.t;
+    var c1:W64.t;
+    var c2:W64.t;
+    var r:W64.t;
+    
+    c1 <- (ctr `>>` (W8.of_int 6));
+    c2 <- (ctr - (c1 * (W64.of_int 64)));
+    r <- kk.[(W64.to_uint c1)];
+    bit <@ ith_bit64 (r, c2);
+    return (bit);
+  }
+  
+  proc swapr (x:W64.t Array4.t, y:W64.t Array4.t, swap_0:W64.t) : W64.t Array4.t *
+                                                                  W64.t Array4.t = {
+    var aux: int;
+    
+    var mask:W64.t;
+    var i:int;
+    var tmp1:W64.t;
+    var tmp2:W64.t;
+    
+    mask <- (swap_0 * (W64.of_int 18446744073709551615));
+    i <- 0;
+    while (i < 4) {
+      tmp1 <- x.[i];
+      tmp1 <- (tmp1 `^` y.[i]);
+      tmp1 <- (tmp1 `&` mask);
+      x.[i] <- (x.[i] `^` tmp1);
+      tmp2 <- y.[i];
+      tmp2 <- (tmp2 `^` tmp1);
+      y.[i] <- tmp2;
+      i <- i + 1;
+    }
+    return (x, y);
+  }
+  
   proc maskOnCarry (mask:int, r:W64.t, _cf:bool) : W64.t = {
     
     
     
-    (_cf, r) <- subc_64 r r _cf;
+    (_cf, r) <- sbb_64 r r _cf;
     r <- (r `&` (W64.of_int mask));
     return (r);
   }
@@ -284,20 +335,19 @@ module M = {
     var twop63:W64.t;
     var cf:bool;
     t <- witness;
-    (* t <- copy_64 x; *)
-     t <- x;
+    t <- copy_64 x;
     twop63 <- (W64.of_int 1);
     twop63 <- (twop63 `<<` (W8.of_int 63));
-    (aux, aux_0) <- addc_64 t.[0] (W64.of_int 19) false;
+    (aux, aux_0) <- adc_64 t.[0] (W64.of_int 19) false;
     cf <- aux;
     t.[0] <- aux_0;
-    (aux, aux_0) <- addc_64 t.[1] (W64.of_int 0) cf;
+    (aux, aux_0) <- adc_64 t.[1] (W64.of_int 0) cf;
     cf <- aux;
     t.[1] <- aux_0;
-    (aux, aux_0) <- addc_64 t.[2] (W64.of_int 0) cf;
+    (aux, aux_0) <- adc_64 t.[2] (W64.of_int 0) cf;
     cf <- aux;
     t.[2] <- aux_0;
-    (aux, aux_0) <- addc_64 t.[3] twop63 cf;
+    (aux, aux_0) <- adc_64 t.[3] twop63 cf;
     cf <- aux;
     t.[3] <- aux_0;
     x.[0] <- (cf ? t.[0] : x.[0]);
@@ -382,7 +432,8 @@ module M = {
     return (g0, g1, g2, g3);
   }
   
-  proc mulm (a:W64.t Array4.t, b:W64.t Array4.t) : W64.t Array4.t = {
+  proc mulm (p:W64.t Array4.t, a:W64.t Array4.t, b:W64.t Array4.t) : 
+  W64.t Array4.t = {
     
     var g0:W64.t;
     var g1:W64.t;
@@ -463,6 +514,64 @@ module M = {
     return (a);
   }
   
+  proc expm (m:W64.t Array4.t, x:W64.t Array4.t, n:W64.t Array4.t) : 
+  W64.t Array4.t = {
+    
+    var x1:W64.t Array4.t;
+    var ctr:W64.t;
+    var x2:W64.t Array4.t;
+    var d:W64.t;
+    var x3:W64.t Array4.t;
+    var x4:W64.t Array4.t;
+    var p:W64.t;
+    var lbit:W64.t;
+    var t1:W64.t;
+    var t2:W64.t;
+    var q:W64.t;
+    var par:W64.t;
+    var cbit:W64.t;
+    x1 <- witness;
+    x2 <- witness;
+    x3 <- witness;
+    x4 <- witness;
+    ctr <- (W64.of_int ((4 * 64) - 1));
+    x1.[0] <- (W64.of_int 1);
+    x1.[1] <- (W64.of_int 0);
+    x1.[2] <- (W64.of_int 0);
+    x1.[3] <- (W64.of_int 0);
+    x2.[0] <- (W64.of_int 1);
+    x2.[1] <- (W64.of_int 0);
+    x2.[2] <- (W64.of_int 0);
+    x2.[3] <- (W64.of_int 0);
+    d <@ ith_bit (n, ctr);
+    x3 <- copy_64 x;
+    x4 <@ mulm (m, x, x);
+    p <- d;
+    (x1, x3) <@ swapr (x1, x3, d);
+    (x2, x4) <@ swapr (x2, x4, d);
+    
+    while (((W64.of_int 0) \ult ctr)) {
+      lbit <- ctr;
+      ctr <- (ctr - (W64.of_int 1));
+      t1 <@ ith_bit (n, lbit);
+      t2 <@ ith_bit (n, ctr);
+      p <- d;
+      q <- d;
+      d <- (d `|` t2);
+      par <- (t1 `^` t2);
+      (x1, x2) <@ swapr (x1, x2, par);
+      x1 <@ mulm (m, x1, x2);
+      x2 <@ mulm (m, x2, x2);
+      q <- (q `|` t2);
+      cbit <- (q `^` p);
+      (x1, x3) <@ swapr (x1, x3, cbit);
+      (x2, x4) <@ swapr (x2, x4, cbit);
+    }
+    par <@ ith_bit (n, (W64.of_int 0));
+    (x1, x2) <@ swapr (x2, x1, par);
+    return (x1);
+  }
+  
   proc toEC () : unit = {
     
     var a:W64.t Array4.t;
@@ -470,12 +579,17 @@ module M = {
     var r:W64.t Array4.t;
     var x:W64.t;
     var _cf:bool;
+    var  _0:W64.t Array4.t;
+     _0 <- witness;
     a <- witness;
     b <- witness;
     r <- witness;
     r <@ addm (a, b);
     r <@ subm (a, b);
-    r <@ mulm (a, b);
+    r <@ mulm (a, a, b);
+    r <@ expm (a, a, b);
+    x <@ ith_bit (a, x);
+    ( _0, a) <@ swapr (a, a, x);
     x <@ bn_eq (a, b);
     x <@ bn_test0 (a);
     _cf <- false;
