w64x4/proof/Fp_w64x4_extract_ct_proof.ec
@@ -1,0 +1,7 @@
+require import Fp_w64x4_extract_ct.
+
+
+equiv fp_w64x4_ct :
+  M.expm ~ M.expm :
+  ={M.leakages, glob M} ==> ={M.leakages}.
+proof. proc; inline *; sim. qed.
