w64x4/src/Fp_w64x4_extract_ct.ec
@@ -1,0 +1,1143 @@
+require import AllCore IntDiv CoreMap List Distr.
+from Jasmin require import JModel.
+
+require import Array4 Array8 Array32.
+require import WArray32 WArray64.
+
+
+
+module M = {
+  var leakages : leakages_t
+  
+  proc bn2_unpack (a:W64.t Array8.t) : W64.t Array4.t * W64.t Array4.t = {
+    var aux: int;
+    var aux_0: W64.t;
+    
+    var hi:W64.t Array4.t;
+    var lo:W64.t Array4.t;
+    var i:int;
+    hi <- witness;
+    lo <- witness;
+    leakages <- LeakFor(0,4) :: LeakAddr([]) :: leakages;
+    i <- 0;
+    while (i < 4) {
+      leakages <- LeakAddr([i]) :: leakages;
+      aux_0 <- a.[i];
+      leakages <- LeakAddr([i]) :: leakages;
+      lo.[i] <- aux_0;
+      leakages <- LeakAddr([(4 + i)]) :: leakages;
+      aux_0 <- a.[(4 + i)];
+      leakages <- LeakAddr([i]) :: leakages;
+      hi.[i] <- aux_0;
+      i <- i + 1;
+    }
+    return (hi, lo);
+  }
+  
+  proc bn_eq (a:W64.t Array4.t, b:W64.t Array4.t) : W64.t = {
+    var aux_5: bool;
+    var aux_4: bool;
+    var aux_3: bool;
+    var aux_2: bool;
+    var aux_1: bool;
+    var aux_0: int;
+    var aux: W64.t;
+    
+    var res_0:W64.t;
+    var are_equal:W64.t;
+    var acc:W64.t;
+    var i:int;
+    var t:W64.t;
+    var zf:bool;
+    var  _0:bool;
+    var  _1:bool;
+    var  _2:bool;
+    var  _3:bool;
+    var  _4:W64.t;
+    
+    leakages <- LeakAddr([]) :: leakages;
+    aux <- (W64.of_int 0);
+    res_0 <- aux;
+    leakages <- LeakAddr([]) :: leakages;
+    aux <- (W64.of_int 1);
+    are_equal <- aux;
+    leakages <- LeakAddr([]) :: leakages;
+    aux <- (W64.of_int 0);
+    acc <- aux;
+    leakages <- LeakFor(0,4) :: LeakAddr([]) :: leakages;
+    i <- 0;
+    while (i < 4) {
+      leakages <- LeakAddr([i]) :: leakages;
+      aux <- a.[i];
+      t <- aux;
+      leakages <- LeakAddr([i]) :: leakages;
+      aux <- (t `^` b.[i]);
+      t <- aux;
+      leakages <- LeakAddr([]) :: leakages;
+      aux <- (acc `|` t);
+      acc <- aux;
+      i <- i + 1;
+    }
+    leakages <- LeakAddr([]) :: leakages;
+    (aux_5, aux_4, aux_3, aux_2, aux_1, aux) <- AND_64 acc acc;
+     _0 <- aux_5;
+     _1 <- aux_4;
+     _2 <- aux_3;
+     _3 <- aux_2;
+    zf <- aux_1;
+     _4 <- aux;
+    leakages <- LeakAddr([]) :: leakages;
+    aux <- (zf ? are_equal : res_0);
+    res_0 <- aux;
+    return (res_0);
+  }
+  
+  proc bn_test0 (a:W64.t Array4.t) : W64.t = {
+    var aux_5: bool;
+    var aux_4: bool;
+    var aux_3: bool;
+    var aux_2: bool;
+    var aux_1: bool;
+    var aux_0: int;
+    var aux: W64.t;
+    
+    var res_0:W64.t;
+    var is_zero:W64.t;
+    var acc:W64.t;
+    var i:int;
+    var zf:bool;
+    var  _0:bool;
+    var  _1:bool;
+    var  _2:bool;
+    var  _3:bool;
+    var  _4:W64.t;
+    
+    leakages <- LeakAddr([]) :: leakages;
+    aux <- (W64.of_int 0);
+    res_0 <- aux;
+    leakages <- LeakAddr([]) :: leakages;
+    aux <- (W64.of_int 1);
+    is_zero <- aux;
+    leakages <- LeakAddr([0]) :: leakages;
+    aux <- a.[0];
+    acc <- aux;
+    leakages <- LeakFor(1,4) :: LeakAddr([]) :: leakages;
+    i <- 1;
+    while (i < 4) {
+      leakages <- LeakAddr([i]) :: leakages;
+      aux <- (acc `|` a.[i]);
+      acc <- aux;
+      i <- i + 1;
+    }
+    leakages <- LeakAddr([]) :: leakages;
+    (aux_5, aux_4, aux_3, aux_2, aux_1, aux) <- AND_64 acc acc;
+     _0 <- aux_5;
+     _1 <- aux_4;
+     _2 <- aux_3;
+     _3 <- aux_2;
+    zf <- aux_1;
+     _4 <- aux;
+    leakages <- LeakAddr([]) :: leakages;
+    aux <- (zf ? is_zero : res_0);
+    res_0 <- aux;
+    return (res_0);
+  }
+  
+  proc bn_add1 (a:W64.t Array4.t, b:W64.t) : bool * W64.t Array4.t = {
+    var aux: bool;
+    var aux_1: int;
+    var aux_0: W64.t;
+    
+    var cf:bool;
+    var i:int;
+    
+    leakages <- LeakAddr([0]) :: leakages;
+    (aux, aux_0) <- adc_64 a.[0] b false;
+    cf <- aux;
+    leakages <- LeakAddr([0]) :: leakages;
+    a.[0] <- aux_0;
+    leakages <- LeakFor(1,4) :: LeakAddr([]) :: leakages;
+    i <- 1;
+    while (i < 4) {
+      leakages <- LeakAddr([i]) :: leakages;
+      (aux, aux_0) <- adc_64 a.[i] (W64.of_int 0) cf;
+      cf <- aux;
+      leakages <- LeakAddr([i]) :: leakages;
+      a.[i] <- aux_0;
+      i <- i + 1;
+    }
+    return (cf, a);
+  }
+  
+  proc bn_addc (a:W64.t Array4.t, b:W64.t Array4.t) : bool * W64.t Array4.t = {
+    var aux: bool;
+    var aux_1: int;
+    var aux_0: W64.t;
+    
+    var cf:bool;
+    var i:int;
+    
+    leakages <- LeakAddr([0; 0]) :: leakages;
+    (aux, aux_0) <- adc_64 a.[0] b.[0] false;
+    cf <- aux;
+    leakages <- LeakAddr([0]) :: leakages;
+    a.[0] <- aux_0;
+    leakages <- LeakFor(1,4) :: LeakAddr([]) :: leakages;
+    i <- 1;
+    while (i < 4) {
+      leakages <- LeakAddr([i; i]) :: leakages;
+      (aux, aux_0) <- adc_64 a.[i] b.[i] cf;
+      cf <- aux;
+      leakages <- LeakAddr([i]) :: leakages;
+      a.[i] <- aux_0;
+      i <- i + 1;
+    }
+    return (cf, a);
+  }
+  
+  proc bn_subc (a:W64.t Array4.t, b:W64.t Array4.t) : bool * W64.t Array4.t = {
+    var aux: bool;
+    var aux_1: int;
+    var aux_0: W64.t;
+    
+    var cf:bool;
+    var i:int;
+    
+    leakages <- LeakAddr([0; 0]) :: leakages;
+    (aux, aux_0) <- sbb_64 a.[0] b.[0] false;
+    cf <- aux;
+    leakages <- LeakAddr([0]) :: leakages;
+    a.[0] <- aux_0;
+    leakages <- LeakFor(1,4) :: LeakAddr([]) :: leakages;
+    i <- 1;
+    while (i < 4) {
+      leakages <- LeakAddr([i; i]) :: leakages;
+      (aux, aux_0) <- sbb_64 a.[i] b.[i] cf;
+      cf <- aux;
+      leakages <- LeakAddr([i]) :: leakages;
+      a.[i] <- aux_0;
+      i <- i + 1;
+    }
+    return (cf, a);
+  }
+  
+  proc mul1 (a:W64.t, b:W64.t Array4.t) : W64.t * bool * bool *
+                                          W64.t Array8.t = {
+    var aux_3: bool;
+    var aux_2: bool;
+    var aux_1: bool;
+    var aux_0: bool;
+    var aux: bool;
+    var aux_6: int;
+    var aux_5: W64.t;
+    var aux_4: W64.t;
+    
+    var _zero:W64.t;
+    var of_0:bool;
+    var cf:bool;
+    var r:W64.t Array8.t;
+    var i:int;
+    var lo:W64.t;
+    var  _0:bool;
+    var  _1:bool;
+    var  _2:bool;
+    r <- witness;
+    leakages <- LeakAddr([]) :: leakages;
+    (aux_3, aux_2, aux_1, aux_0, aux, aux_5) <- set0_64 ;
+    of_0 <- aux_3;
+    cf <- aux_2;
+     _0 <- aux_1;
+     _1 <- aux_0;
+     _2 <- aux;
+    _zero <- aux_5;
+    leakages <- LeakAddr([0]) :: leakages;
+    (aux_5, aux_4) <- MULX_64 a b.[0];
+    leakages <- LeakAddr([1]) :: leakages;
+    r.[1] <- aux_5;
+    leakages <- LeakAddr([0]) :: leakages;
+    r.[0] <- aux_4;
+    leakages <- LeakFor(1,4) :: LeakAddr([]) :: leakages;
+    i <- 1;
+    while (i < 4) {
+      leakages <- LeakAddr([i]) :: leakages;
+      (aux_5, aux_4) <- MULX_64 a b.[i];
+      leakages <- LeakAddr([(i + 1)]) :: leakages;
+      r.[(i + 1)] <- aux_5;
+      lo <- aux_4;
+      leakages <- LeakAddr([i]) :: leakages;
+      (aux_3, aux_5) <- ADCX_64 r.[i] lo cf;
+      cf <- aux_3;
+      leakages <- LeakAddr([i]) :: leakages;
+      r.[i] <- aux_5;
+      i <- i + 1;
+    }
+    leakages <- LeakAddr([4]) :: leakages;
+    (aux_3, aux_5) <- ADCX_64 r.[4] _zero cf;
+    cf <- aux_3;
+    leakages <- LeakAddr([4]) :: leakages;
+    r.[4] <- aux_5;
+    return (_zero, of_0, cf, r);
+  }
+  
+  proc mul1acc (k:int, a:W64.t, b:W64.t Array4.t, r:W64.t Array8.t,
+                _zero:W64.t, of_0:bool, cf:bool) : W64.t * bool * bool *
+                                                   W64.t Array8.t = {
+    var aux_2: bool;
+    var aux: int;
+    var aux_1: W64.t;
+    var aux_0: W64.t;
+    
+    var i:int;
+    var hi:W64.t;
+    var lo:W64.t;
+    
+    leakages <- LeakFor(0,(4 - 1)) :: LeakAddr([]) :: leakages;
+    aux <- (4 - 1);
+    i <- 0;
+    while (i < aux) {
+      leakages <- LeakAddr([i]) :: leakages;
+      (aux_1, aux_0) <- MULX_64 a b.[i];
+      hi <- aux_1;
+      lo <- aux_0;
+      leakages <- LeakAddr([(k + i)]) :: leakages;
+      (aux_2, aux_1) <- ADOX_64 r.[(k + i)] lo of_0;
+      of_0 <- aux_2;
+      leakages <- LeakAddr([(k + i)]) :: leakages;
+      r.[(k + i)] <- aux_1;
+      leakages <- LeakAddr([((k + i) + 1)]) :: leakages;
+      (aux_2, aux_1) <- ADCX_64 r.[((k + i) + 1)] hi cf;
+      cf <- aux_2;
+      leakages <- LeakAddr([((k + i) + 1)]) :: leakages;
+      r.[((k + i) + 1)] <- aux_1;
+      i <- i + 1;
+    }
+    leakages <- LeakAddr([(4 - 1)]) :: leakages;
+    (aux_1, aux_0) <- MULX_64 a b.[(4 - 1)];
+    leakages <- LeakAddr([(4 + k)]) :: leakages;
+    r.[(4 + k)] <- aux_1;
+    lo <- aux_0;
+    leakages <- LeakAddr([((4 + k) - 1)]) :: leakages;
+    (aux_2, aux_1) <- ADOX_64 r.[((4 + k) - 1)] lo of_0;
+    of_0 <- aux_2;
+    leakages <- LeakAddr([((4 + k) - 1)]) :: leakages;
+    r.[((4 + k) - 1)] <- aux_1;
+    leakages <- LeakAddr([(4 + k)]) :: leakages;
+    (aux_2, aux_1) <- ADCX_64 r.[(4 + k)] _zero cf;
+    cf <- aux_2;
+    leakages <- LeakAddr([(4 + k)]) :: leakages;
+    r.[(4 + k)] <- aux_1;
+    leakages <- LeakAddr([(4 + k)]) :: leakages;
+    (aux_2, aux_1) <- ADOX_64 r.[(4 + k)] _zero of_0;
+    of_0 <- aux_2;
+    leakages <- LeakAddr([(4 + k)]) :: leakages;
+    r.[(4 + k)] <- aux_1;
+    return (_zero, of_0, cf, r);
+  }
+  
+  proc bn_muln (a:W64.t Array4.t, b:W64.t Array4.t) : W64.t * bool * bool *
+                                                      W64.t Array8.t = {
+    var aux_1: bool;
+    var aux_0: bool;
+    var aux_3: int;
+    var aux: W64.t;
+    var aux_2: W64.t Array8.t;
+    
+    var _zero:W64.t;
+    var of_0:bool;
+    var cf:bool;
+    var r:W64.t Array8.t;
+    var ai:W64.t;
+    var i:int;
+    r <- witness;
+    leakages <- LeakAddr([0]) :: leakages;
+    aux <- a.[0];
+    ai <- aux;
+    leakages <- LeakAddr([]) :: leakages;
+    (aux, aux_1, aux_0, aux_2) <@ mul1 (ai, b);
+    _zero <- aux;
+    of_0 <- aux_1;
+    cf <- aux_0;
+    r <- aux_2;
+    leakages <- LeakFor(1,4) :: LeakAddr([]) :: leakages;
+    i <- 1;
+    while (i < 4) {
+      leakages <- LeakAddr([i]) :: leakages;
+      aux <- a.[i];
+      ai <- aux;
+      leakages <- LeakAddr([]) :: leakages;
+      (aux, aux_1, aux_0, aux_2) <@ mul1acc (i, ai, b, r, _zero, of_0, cf);
+      _zero <- aux;
+      of_0 <- aux_1;
+      cf <- aux_0;
+      r <- aux_2;
+      i <- i + 1;
+    }
+    return (_zero, of_0, cf, r);
+  }
+  
+  proc ith_bit64 (k:W64.t, ctr:W64.t) : W64.t = {
+    var aux: W64.t;
+    
+    var bit:W64.t;
+    var p:W64.t;
+    
+    leakages <- LeakAddr([]) :: leakages;
+    aux <- k;
+    bit <- aux;
+    leakages <- LeakAddr([]) :: leakages;
+    aux <- ctr;
+    p <- aux;
+    leakages <- LeakAddr([]) :: leakages;
+    aux <- (p `&` (W64.of_int 63));
+    p <- aux;
+    leakages <- LeakAddr([]) :: leakages;
+    aux <- (bit `>>` (truncateu8 p));
+    bit <- aux;
+    leakages <- LeakAddr([]) :: leakages;
+    aux <- (bit `&` (W64.of_int 1));
+    bit <- aux;
+    return (bit);
+  }
+  
+  proc ith_bit (kk:W64.t Array4.t, ctr:W64.t) : W64.t = {
+    var aux: W64.t;
+    
+    var bit:W64.t;
+    var c1:W64.t;
+    var c2:W64.t;
+    var r:W64.t;
+    
+    leakages <- LeakAddr([]) :: leakages;
+    aux <- (ctr `>>` (W8.of_int 6));
+    c1 <- aux;
+    leakages <- LeakAddr([]) :: leakages;
+    aux <- (ctr - (c1 * (W64.of_int 64)));
+    c2 <- aux;
+    leakages <- LeakAddr([(W64.to_uint c1)]) :: leakages;
+    aux <- kk.[(W64.to_uint c1)];
+    r <- aux;
+    leakages <- LeakAddr([]) :: leakages;
+    aux <@ ith_bit64 (r, c2);
+    bit <- aux;
+    return (bit);
+  }
+  
+  proc swapr (x:W64.t Array4.t, y:W64.t Array4.t, swap_0:W64.t) : W64.t Array4.t *
+                                                                  W64.t Array4.t = {
+    var aux_0: int;
+    var aux: W64.t;
+    
+    var mask:W64.t;
+    var i:int;
+    var tmp1:W64.t;
+    var tmp2:W64.t;
+    
+    leakages <- LeakAddr([]) :: leakages;
+    aux <- (swap_0 * (W64.of_int 18446744073709551615));
+    mask <- aux;
+    leakages <- LeakFor(0,4) :: LeakAddr([]) :: leakages;
+    i <- 0;
+    while (i < 4) {
+      leakages <- LeakAddr([i]) :: leakages;
+      aux <- x.[i];
+      tmp1 <- aux;
+      leakages <- LeakAddr([i]) :: leakages;
+      aux <- (tmp1 `^` y.[i]);
+      tmp1 <- aux;
+      leakages <- LeakAddr([]) :: leakages;
+      aux <- (tmp1 `&` mask);
+      tmp1 <- aux;
+      leakages <- LeakAddr([i]) :: leakages;
+      aux <- (x.[i] `^` tmp1);
+      leakages <- LeakAddr([i]) :: leakages;
+      x.[i] <- aux;
+      leakages <- LeakAddr([i]) :: leakages;
+      aux <- y.[i];
+      tmp2 <- aux;
+      leakages <- LeakAddr([]) :: leakages;
+      aux <- (tmp2 `^` tmp1);
+      tmp2 <- aux;
+      leakages <- LeakAddr([]) :: leakages;
+      aux <- tmp2;
+      leakages <- LeakAddr([i]) :: leakages;
+      y.[i] <- aux;
+      i <- i + 1;
+    }
+    return (x, y);
+  }
+  
+  proc maskOnCarry (mask:int, r:W64.t, _cf:bool) : W64.t = {
+    var aux: bool;
+    var aux_0: W64.t;
+    
+    
+    
+    leakages <- LeakAddr([]) :: leakages;
+    (aux, aux_0) <- sbb_64 r r _cf;
+    _cf <- aux;
+    r <- aux_0;
+    leakages <- LeakAddr([]) :: leakages;
+    aux_0 <- (r `&` (W64.of_int mask));
+    r <- aux_0;
+    return (r);
+  }
+  
+  proc x2r (x0:W64.t, x1:W64.t, x2:W64.t, x3:W64.t) : W64.t Array4.t = {
+    var aux: W64.t;
+    
+    var r:W64.t Array4.t;
+    r <- witness;
+    leakages <- LeakAddr([]) :: leakages;
+    aux <- x0;
+    leakages <- LeakAddr([0]) :: leakages;
+    r.[0] <- aux;
+    leakages <- LeakAddr([]) :: leakages;
+    aux <- x1;
+    leakages <- LeakAddr([1]) :: leakages;
+    r.[1] <- aux;
+    leakages <- LeakAddr([]) :: leakages;
+    aux <- x2;
+    leakages <- LeakAddr([2]) :: leakages;
+    r.[2] <- aux;
+    leakages <- LeakAddr([]) :: leakages;
+    aux <- x3;
+    leakages <- LeakAddr([3]) :: leakages;
+    r.[3] <- aux;
+    return (r);
+  }
+  
+  proc r2x (x:W64.t Array4.t) : W64.t * W64.t * W64.t * W64.t = {
+    var aux: W64.t;
+    
+    var r0:W64.t;
+    var r1:W64.t;
+    var r2:W64.t;
+    var r3:W64.t;
+    
+    leakages <- LeakAddr([0]) :: leakages;
+    aux <- x.[0];
+    r0 <- aux;
+    leakages <- LeakAddr([1]) :: leakages;
+    aux <- x.[1];
+    r1 <- aux;
+    leakages <- LeakAddr([2]) :: leakages;
+    aux <- x.[2];
+    r2 <- aux;
+    leakages <- LeakAddr([3]) :: leakages;
+    aux <- x.[3];
+    r3 <- aux;
+    return (r0, r1, r2, r3);
+  }
+  
+  proc cminusP (x:W64.t Array4.t) : W64.t Array4.t = {
+    var aux_2: bool;
+    var aux_1: W64.t;
+    var aux: W8.t Array32.t;
+    var aux_0: W64.t Array4.t;
+    
+    var t:W64.t Array4.t;
+    var twop63:W64.t;
+    var cf:bool;
+    t <- witness;
+    leakages <- LeakAddr([]) :: leakages;
+    aux_0 <- copy_64 x;
+    t <- aux_0;
+    leakages <- LeakAddr([]) :: leakages;
+    aux_1 <- (W64.of_int 1);
+    twop63 <- aux_1;
+    leakages <- LeakAddr([]) :: leakages;
+    aux_1 <- (twop63 `<<` (W8.of_int 63));
+    twop63 <- aux_1;
+    leakages <- LeakAddr([0]) :: leakages;
+    (aux_2, aux_1) <- adc_64 t.[0] (W64.of_int 19) false;
+    cf <- aux_2;
+    leakages <- LeakAddr([0]) :: leakages;
+    t.[0] <- aux_1;
+    leakages <- LeakAddr([1]) :: leakages;
+    (aux_2, aux_1) <- adc_64 t.[1] (W64.of_int 0) cf;
+    cf <- aux_2;
+    leakages <- LeakAddr([1]) :: leakages;
+    t.[1] <- aux_1;
+    leakages <- LeakAddr([2]) :: leakages;
+    (aux_2, aux_1) <- adc_64 t.[2] (W64.of_int 0) cf;
+    cf <- aux_2;
+    leakages <- LeakAddr([2]) :: leakages;
+    t.[2] <- aux_1;
+    leakages <- LeakAddr([3]) :: leakages;
+    (aux_2, aux_1) <- adc_64 t.[3] twop63 cf;
+    cf <- aux_2;
+    leakages <- LeakAddr([3]) :: leakages;
+    t.[3] <- aux_1;
+    leakages <- LeakAddr([0; 0]) :: leakages;
+    aux_1 <- (cf ? t.[0] : x.[0]);
+    leakages <- LeakAddr([0]) :: leakages;
+    x.[0] <- aux_1;
+    leakages <- LeakAddr([1; 1]) :: leakages;
+    aux_1 <- (cf ? t.[1] : x.[1]);
+    leakages <- LeakAddr([1]) :: leakages;
+    x.[1] <- aux_1;
+    leakages <- LeakAddr([2; 2]) :: leakages;
+    aux_1 <- (cf ? t.[2] : x.[2]);
+    leakages <- LeakAddr([2]) :: leakages;
+    x.[2] <- aux_1;
+    leakages <- LeakAddr([3; 3]) :: leakages;
+    aux_1 <- (cf ? t.[3] : x.[3]);
+    leakages <- LeakAddr([3]) :: leakages;
+    x.[3] <- aux_1;
+    return (x);
+  }
+  
+  proc caddP (cf:bool, x:W64.t Array4.t) : W64.t Array4.t = {
+    var aux_0: bool;
+    var aux: W64.t;
+    var aux_1: W64.t Array4.t;
+    
+    var p:W64.t Array4.t;
+    var _zero:W64.t;
+    var  _0:bool;
+    p <- witness;
+    leakages <- LeakAddr([]) :: leakages;
+    aux <- (W64.of_int 18446744073709551597);
+    leakages <- LeakAddr([0]) :: leakages;
+    p.[0] <- aux;
+    leakages <- LeakAddr([]) :: leakages;
+    aux <- (W64.of_int 18446744073709551615);
+    leakages <- LeakAddr([1]) :: leakages;
+    p.[1] <- aux;
+    leakages <- LeakAddr([]) :: leakages;
+    aux <- (W64.of_int 18446744073709551615);
+    leakages <- LeakAddr([2]) :: leakages;
+    p.[2] <- aux;
+    leakages <- LeakAddr([]) :: leakages;
+    aux <- (W64.of_int 9223372036854775807);
+    leakages <- LeakAddr([3]) :: leakages;
+    p.[3] <- aux;
+    leakages <- LeakAddr([]) :: leakages;
+    aux <- (W64.of_int 0);
+    _zero <- aux;
+    leakages <- LeakAddr([0]) :: leakages;
+    aux <- ((! cf) ? _zero : p.[0]);
+    leakages <- LeakAddr([0]) :: leakages;
+    p.[0] <- aux;
+    leakages <- LeakAddr([1]) :: leakages;
+    aux <- ((! cf) ? _zero : p.[1]);
+    leakages <- LeakAddr([1]) :: leakages;
+    p.[1] <- aux;
+    leakages <- LeakAddr([2]) :: leakages;
+    aux <- ((! cf) ? _zero : p.[2]);
+    leakages <- LeakAddr([2]) :: leakages;
+    p.[2] <- aux;
+    leakages <- LeakAddr([3]) :: leakages;
+    aux <- ((! cf) ? _zero : p.[3]);
+    leakages <- LeakAddr([3]) :: leakages;
+    p.[3] <- aux;
+    leakages <- LeakAddr([]) :: leakages;
+    (aux_0, aux_1) <@ bn_addc (x, p);
+     _0 <- aux_0;
+    x <- aux_1;
+    return (x);
+  }
+  
+  proc redp25519 (_of:bool, _cf:bool, a:W64.t Array8.t) : W64.t Array4.t = {
+    var aux_7: bool;
+    var aux_6: bool;
+    var aux_5: bool;
+    var aux_3: bool;
+    var aux_2: bool;
+    var aux: W64.t;
+    var aux_1: W64.t Array4.t;
+    var aux_0: W64.t Array4.t;
+    var aux_4: W64.t Array8.t;
+    
+    var al:W64.t Array4.t;
+    var tmp:W64.t;
+    var _zero:W64.t;
+    var ah:W64.t Array4.t;
+    var  _0:W64.t Array4.t;
+    var  _1:bool;
+    var  _2:bool;
+    var  _3:bool;
+    var  _4:bool;
+    var  _5:bool;
+    var  _6:W64.t Array4.t;
+     _0 <- witness;
+     _6 <- witness;
+    ah <- witness;
+    al <- witness;
+    leakages <- LeakAddr([]) :: leakages;
+    aux <- (W64.of_int 38);
+    tmp <- aux;
+    leakages <- LeakAddr([]) :: leakages;
+    aux <- (W64.of_int 0);
+    _zero <- aux;
+    leakages <- LeakAddr([]) :: leakages;
+    (aux_1, aux_0) <@ bn2_unpack (a);
+    ah <- aux_1;
+     _0 <- aux_0;
+    leakages <- LeakAddr([]) :: leakages;
+    (aux, aux_7, aux_6, aux_4) <@ mul1acc (0, tmp, ah, a, _zero, _of, _cf);
+    _zero <- aux;
+    _of <- aux_7;
+    _cf <- aux_6;
+    a <- aux_4;
+    leakages <- LeakAddr([4]) :: leakages;
+    (aux_7, aux_6, aux_5, aux_3, aux_2, aux) <- IMULri_64 a.[4]
+    (W64.of_int 38);
+     _1 <- aux_7;
+     _2 <- aux_6;
+     _3 <- aux_5;
+     _4 <- aux_3;
+     _5 <- aux_2;
+    tmp <- aux;
+    leakages <- LeakAddr([]) :: leakages;
+    (aux_1, aux_0) <@ bn2_unpack (a);
+     _6 <- aux_1;
+    al <- aux_0;
+    leakages <- LeakAddr([]) :: leakages;
+    (aux_7, aux_1) <@ bn_add1 (al, tmp);
+    _cf <- aux_7;
+    al <- aux_1;
+    leakages <- LeakAddr([]) :: leakages;
+    aux <@ maskOnCarry (38, tmp, _cf);
+    tmp <- aux;
+    leakages <- LeakAddr([0]) :: leakages;
+    aux <- (al.[0] + tmp);
+    leakages <- LeakAddr([0]) :: leakages;
+    al.[0] <- aux;
+    return (al);
+  }
+  
+  proc freeze (x:W64.t Array4.t) : W64.t Array4.t = {
+    var aux: W64.t Array4.t;
+    
+    
+    
+    leakages <- LeakAddr([]) :: leakages;
+    aux <@ cminusP (x);
+    x <- aux;
+    leakages <- LeakAddr([]) :: leakages;
+    aux <@ cminusP (x);
+    x <- aux;
+    return (x);
+  }
+  
+  proc _mulm (f:W64.t Array4.t, g0:W64.t, g1:W64.t, g2:W64.t, g3:W64.t) : 
+  W64.t * W64.t * W64.t * W64.t = {
+    var aux_2: bool;
+    var aux_1: bool;
+    var aux_6: W64.t;
+    var aux_5: W64.t;
+    var aux_4: W64.t;
+    var aux_0: W64.t;
+    var aux: W64.t Array4.t;
+    var aux_3: W64.t Array8.t;
+    
+    var g:W64.t Array4.t;
+    var _zero:W64.t;
+    var of_0:bool;
+    var cf:bool;
+    var h:W64.t Array8.t;
+    g <- witness;
+    h <- witness;
+    leakages <- LeakAddr([]) :: leakages;
+    aux <@ x2r (g0, g1, g2, g3);
+    g <- aux;
+    leakages <- LeakAddr([]) :: leakages;
+    (aux_6, aux_2, aux_1, aux_3) <@ bn_muln (f, g);
+    _zero <- aux_6;
+    of_0 <- aux_2;
+    cf <- aux_1;
+    h <- aux_3;
+    leakages <- LeakAddr([]) :: leakages;
+    aux <@ redp25519 (of_0, cf, h);
+    g <- aux;
+    leakages <- LeakAddr([]) :: leakages;
+    aux <@ freeze (g);
+    g <- aux;
+    leakages <- LeakAddr([]) :: leakages;
+    (aux_6, aux_5, aux_4, aux_0) <@ r2x (g);
+    g0 <- aux_6;
+    g1 <- aux_5;
+    g2 <- aux_4;
+    g3 <- aux_0;
+    return (g0, g1, g2, g3);
+  }
+  
+  proc mulm (p:W64.t Array4.t, a:W64.t Array4.t, b:W64.t Array4.t) : 
+  W64.t Array4.t = {
+    var aux_2: W64.t;
+    var aux_1: W64.t;
+    var aux_0: W64.t;
+    var aux: W64.t;
+    var aux_3: W64.t Array4.t;
+    
+    var g0:W64.t;
+    var g1:W64.t;
+    var g2:W64.t;
+    var g3:W64.t;
+    
+    leakages <- LeakAddr([]) :: leakages;
+    (aux_2, aux_1, aux_0, aux) <@ r2x (b);
+    g0 <- aux_2;
+    g1 <- aux_1;
+    g2 <- aux_0;
+    g3 <- aux;
+    leakages <- LeakAddr([]) :: leakages;
+    (aux_2, aux_1, aux_0, aux) <@ _mulm (a, g0, g1, g2, g3);
+    g0 <- aux_2;
+    g1 <- aux_1;
+    g2 <- aux_0;
+    g3 <- aux;
+    leakages <- LeakAddr([]) :: leakages;
+    aux_3 <@ x2r (g0, g1, g2, g3);
+    b <- aux_3;
+    return (b);
+  }
+  
+  proc _addm (f0:W64.t, f1:W64.t, f2:W64.t, f3:W64.t, g0:W64.t, g1:W64.t,
+              g2:W64.t, g3:W64.t) : W64.t * W64.t * W64.t * W64.t = {
+    var aux_0: bool;
+    var aux_4: W64.t;
+    var aux_3: W64.t;
+    var aux_2: W64.t;
+    var aux_1: W64.t;
+    var aux: W64.t Array4.t;
+    
+    var f:W64.t Array4.t;
+    var g:W64.t Array4.t;
+    var  _0:bool;
+    f <- witness;
+    g <- witness;
+    leakages <- LeakAddr([]) :: leakages;
+    aux <@ x2r (f0, f1, f2, f3);
+    f <- aux;
+    leakages <- LeakAddr([]) :: leakages;
+    aux <@ x2r (g0, g1, g2, g3);
+    g <- aux;
+    leakages <- LeakAddr([]) :: leakages;
+    (aux_0, aux) <@ bn_addc (f, g);
+     _0 <- aux_0;
+    f <- aux;
+    leakages <- LeakAddr([]) :: leakages;
+    aux <@ cminusP (f);
+    f <- aux;
+    leakages <- LeakAddr([]) :: leakages;
+    (aux_4, aux_3, aux_2, aux_1) <@ r2x (f);
+    f0 <- aux_4;
+    f1 <- aux_3;
+    f2 <- aux_2;
+    f3 <- aux_1;
+    return (f0, f1, f2, f3);
+  }
+  
+  proc addm (a:W64.t Array4.t, b:W64.t Array4.t) : W64.t Array4.t = {
+    var aux_2: W64.t;
+    var aux_1: W64.t;
+    var aux_0: W64.t;
+    var aux: W64.t;
+    var aux_3: W64.t Array4.t;
+    
+    var f0:W64.t;
+    var f1:W64.t;
+    var f2:W64.t;
+    var f3:W64.t;
+    var g0:W64.t;
+    var g1:W64.t;
+    var g2:W64.t;
+    var g3:W64.t;
+    
+    leakages <- LeakAddr([]) :: leakages;
+    (aux_2, aux_1, aux_0, aux) <@ r2x (a);
+    f0 <- aux_2;
+    f1 <- aux_1;
+    f2 <- aux_0;
+    f3 <- aux;
+    leakages <- LeakAddr([]) :: leakages;
+    (aux_2, aux_1, aux_0, aux) <@ r2x (b);
+    g0 <- aux_2;
+    g1 <- aux_1;
+    g2 <- aux_0;
+    g3 <- aux;
+    leakages <- LeakAddr([]) :: leakages;
+    (aux_2, aux_1, aux_0, aux) <@ _addm (f0, f1, f2, f3, g0, g1, g2, g3);
+    f0 <- aux_2;
+    f1 <- aux_1;
+    f2 <- aux_0;
+    f3 <- aux;
+    leakages <- LeakAddr([]) :: leakages;
+    aux_3 <@ x2r (f0, f1, f2, f3);
+    a <- aux_3;
+    return (a);
+  }
+  
+  proc _subm (f0:W64.t, f1:W64.t, f2:W64.t, f3:W64.t, g0:W64.t, g1:W64.t,
+              g2:W64.t, g3:W64.t) : W64.t * W64.t * W64.t * W64.t = {
+    var aux_0: bool;
+    var aux_4: W64.t;
+    var aux_3: W64.t;
+    var aux_2: W64.t;
+    var aux_1: W64.t;
+    var aux: W64.t Array4.t;
+    
+    var f:W64.t Array4.t;
+    var g:W64.t Array4.t;
+    var cf:bool;
+    f <- witness;
+    g <- witness;
+    leakages <- LeakAddr([]) :: leakages;
+    aux <@ x2r (f0, f1, f2, f3);
+    f <- aux;
+    leakages <- LeakAddr([]) :: leakages;
+    aux <@ x2r (g0, g1, g2, g3);
+    g <- aux;
+    leakages <- LeakAddr([]) :: leakages;
+    (aux_0, aux) <@ bn_subc (f, g);
+    cf <- aux_0;
+    f <- aux;
+    leakages <- LeakAddr([]) :: leakages;
+    aux <@ caddP (cf, f);
+    f <- aux;
+    leakages <- LeakAddr([]) :: leakages;
+    (aux_4, aux_3, aux_2, aux_1) <@ r2x (f);
+    f0 <- aux_4;
+    f1 <- aux_3;
+    f2 <- aux_2;
+    f3 <- aux_1;
+    return (f0, f1, f2, f3);
+  }
+  
+  proc subm (a:W64.t Array4.t, b:W64.t Array4.t) : W64.t Array4.t = {
+    var aux_2: W64.t;
+    var aux_1: W64.t;
+    var aux_0: W64.t;
+    var aux: W64.t;
+    var aux_3: W64.t Array4.t;
+    
+    var f0:W64.t;
+    var f1:W64.t;
+    var f2:W64.t;
+    var f3:W64.t;
+    var g0:W64.t;
+    var g1:W64.t;
+    var g2:W64.t;
+    var g3:W64.t;
+    
+    leakages <- LeakAddr([]) :: leakages;
+    (aux_2, aux_1, aux_0, aux) <@ r2x (a);
+    f0 <- aux_2;
+    f1 <- aux_1;
+    f2 <- aux_0;
+    f3 <- aux;
+    leakages <- LeakAddr([]) :: leakages;
+    (aux_2, aux_1, aux_0, aux) <@ r2x (b);
+    g0 <- aux_2;
+    g1 <- aux_1;
+    g2 <- aux_0;
+    g3 <- aux;
+    leakages <- LeakAddr([]) :: leakages;
+    (aux_2, aux_1, aux_0, aux) <@ _subm (f0, f1, f2, f3, g0, g1, g2, g3);
+    f0 <- aux_2;
+    f1 <- aux_1;
+    f2 <- aux_0;
+    f3 <- aux;
+    leakages <- LeakAddr([]) :: leakages;
+    aux_3 <@ x2r (f0, f1, f2, f3);
+    a <- aux_3;
+    return (a);
+  }
+  
+  proc expm (m:W64.t Array4.t, x:W64.t Array4.t, n:W64.t Array4.t) : 
+  W64.t Array4.t = {
+    var aux: W64.t;
+    var aux_0: W8.t Array32.t;
+    var aux_2: W64.t Array4.t;
+    var aux_1: W64.t Array4.t;
+    
+    var x1:W64.t Array4.t;
+    var ctr:W64.t;
+    var x2:W64.t Array4.t;
+    var d:W64.t;
+    var x3:W64.t Array4.t;
+    var x4:W64.t Array4.t;
+    var p:W64.t;
+    var lbit:W64.t;
+    var t1:W64.t;
+    var t2:W64.t;
+    var q:W64.t;
+    var par:W64.t;
+    var cbit:W64.t;
+    x1 <- witness;
+    x2 <- witness;
+    x3 <- witness;
+    x4 <- witness;
+    leakages <- LeakAddr([]) :: leakages;
+    aux <- (W64.of_int ((4 * 64) - 1));
+    ctr <- aux;
+    leakages <- LeakAddr([]) :: leakages;
+    aux <- (W64.of_int 1);
+    leakages <- LeakAddr([0]) :: leakages;
+    x1.[0] <- aux;
+    leakages <- LeakAddr([]) :: leakages;
+    aux <- (W64.of_int 0);
+    leakages <- LeakAddr([1]) :: leakages;
+    x1.[1] <- aux;
+    leakages <- LeakAddr([]) :: leakages;
+    aux <- (W64.of_int 0);
+    leakages <- LeakAddr([2]) :: leakages;
+    x1.[2] <- aux;
+    leakages <- LeakAddr([]) :: leakages;
+    aux <- (W64.of_int 0);
+    leakages <- LeakAddr([3]) :: leakages;
+    x1.[3] <- aux;
+    leakages <- LeakAddr([]) :: leakages;
+    aux <- (W64.of_int 1);
+    leakages <- LeakAddr([0]) :: leakages;
+    x2.[0] <- aux;
+    leakages <- LeakAddr([]) :: leakages;
+    aux <- (W64.of_int 0);
+    leakages <- LeakAddr([1]) :: leakages;
+    x2.[1] <- aux;
+    leakages <- LeakAddr([]) :: leakages;
+    aux <- (W64.of_int 0);
+    leakages <- LeakAddr([2]) :: leakages;
+    x2.[2] <- aux;
+    leakages <- LeakAddr([]) :: leakages;
+    aux <- (W64.of_int 0);
+    leakages <- LeakAddr([3]) :: leakages;
+    x2.[3] <- aux;
+    leakages <- LeakAddr([]) :: leakages;
+    aux <@ ith_bit (n, ctr);
+    d <- aux;
+    leakages <- LeakAddr([]) :: leakages;
+    aux_2 <- copy_64 x;
+    x3 <- aux_2;
+    leakages <- LeakAddr([]) :: leakages;
+    aux_2 <@ mulm (m, x, x);
+    x4 <- aux_2;
+    leakages <- LeakAddr([]) :: leakages;
+    aux <- d;
+    p <- aux;
+    leakages <- LeakAddr([]) :: leakages;
+    (aux_2, aux_1) <@ swapr (x1, x3, d);
+    x1 <- aux_2;
+    x3 <- aux_1;
+    leakages <- LeakAddr([]) :: leakages;
+    (aux_2, aux_1) <@ swapr (x2, x4, d);
+    x2 <- aux_2;
+    x4 <- aux_1;
+    
+    leakages <- LeakCond(((W64.of_int 0) \ult ctr)) :: LeakAddr([]) :: leakages;
+    
+    while (((W64.of_int 0) \ult ctr)) {
+      leakages <- LeakAddr([]) :: leakages;
+      aux <- ctr;
+      lbit <- aux;
+      leakages <- LeakAddr([]) :: leakages;
+      aux <- (ctr - (W64.of_int 1));
+      ctr <- aux;
+      leakages <- LeakAddr([]) :: leakages;
+      aux <@ ith_bit (n, lbit);
+      t1 <- aux;
+      leakages <- LeakAddr([]) :: leakages;
+      aux <@ ith_bit (n, ctr);
+      t2 <- aux;
+      leakages <- LeakAddr([]) :: leakages;
+      aux <- d;
+      p <- aux;
+      leakages <- LeakAddr([]) :: leakages;
+      aux <- d;
+      q <- aux;
+      leakages <- LeakAddr([]) :: leakages;
+      aux <- (d `|` t2);
+      d <- aux;
+      leakages <- LeakAddr([]) :: leakages;
+      aux <- (t1 `^` t2);
+      par <- aux;
+      leakages <- LeakAddr([]) :: leakages;
+      (aux_2, aux_1) <@ swapr (x1, x2, par);
+      x1 <- aux_2;
+      x2 <- aux_1;
+      leakages <- LeakAddr([]) :: leakages;
+      aux_2 <@ mulm (m, x1, x2);
+      x1 <- aux_2;
+      leakages <- LeakAddr([]) :: leakages;
+      aux_2 <@ mulm (m, x2, x2);
+      x2 <- aux_2;
+      leakages <- LeakAddr([]) :: leakages;
+      aux <- (q `|` t2);
+      q <- aux;
+      leakages <- LeakAddr([]) :: leakages;
+      aux <- (q `^` p);
+      cbit <- aux;
+      leakages <- LeakAddr([]) :: leakages;
+      (aux_2, aux_1) <@ swapr (x1, x3, cbit);
+      x1 <- aux_2;
+      x3 <- aux_1;
+      leakages <- LeakAddr([]) :: leakages;
+      (aux_2, aux_1) <@ swapr (x2, x4, cbit);
+      x2 <- aux_2;
+      x4 <- aux_1;
+    leakages <- LeakCond(((W64.of_int 0) \ult ctr)) :: LeakAddr([]) :: leakages;
+    
+    }
+    leakages <- LeakAddr([]) :: leakages;
+    aux <@ ith_bit (n, (W64.of_int 0));
+    par <- aux;
+    leakages <- LeakAddr([]) :: leakages;
+    (aux_2, aux_1) <@ swapr (x2, x1, par);
+    x1 <- aux_2;
+    x2 <- aux_1;
+    return (x1);
+  }
+  
+  proc toEC () : unit = {
+    var aux_2: bool;
+    var aux_0: W64.t;
+    var aux_1: W64.t Array4.t;
+    var aux: W64.t Array4.t;
+    
+    var a:W64.t Array4.t;
+    var b:W64.t Array4.t;
+    var r:W64.t Array4.t;
+    var x:W64.t;
+    var _cf:bool;
+    var  _0:W64.t Array4.t;
+     _0 <- witness;
+    a <- witness;
+    b <- witness;
+    r <- witness;
+    leakages <- LeakAddr([]) :: leakages;
+    aux_1 <@ addm (a, b);
+    r <- aux_1;
+    leakages <- LeakAddr([]) :: leakages;
+    aux_1 <@ subm (a, b);
+    r <- aux_1;
+    leakages <- LeakAddr([]) :: leakages;
+    aux_1 <@ mulm (a, a, b);
+    r <- aux_1;
+    leakages <- LeakAddr([]) :: leakages;
+    aux_1 <@ expm (a, a, b);
+    r <- aux_1;
+    leakages <- LeakAddr([]) :: leakages;
+    aux_0 <@ ith_bit (a, x);
+    x <- aux_0;
+    leakages <- LeakAddr([]) :: leakages;
+    (aux_1, aux) <@ swapr (a, a, x);
+     _0 <- aux_1;
+    a <- aux;
+    leakages <- LeakAddr([]) :: leakages;
+    aux_0 <@ bn_eq (a, b);
+    x <- aux_0;
+    leakages <- LeakAddr([]) :: leakages;
+    aux_0 <@ bn_test0 (a);
+    x <- aux_0;
+    leakages <- LeakAddr([]) :: leakages;
+    aux_2 <- false;
+    _cf <- aux_2;
+    leakages <- LeakAddr([]) :: leakages;
+    aux_0 <@ maskOnCarry (7, x, _cf);
+    x <- aux_0;
+    return ();
+  }
+}.
+
